M4wp.fst
@@ -1,0 +1,29 @@
+module M4wp
+
+open Common
+open IOStHist
+
+let m4wp_invariant_pre (pi_check : monitorable_prop) (s0:events_trace) : Type0 =
+  enforced_globally default_check s0 &&
+  enforced_globally pi_check s0
+
+let m4wp_invariant_post
+  (#a:Type)
+  (pi_check : monitorable_prop)
+  (s0:events_trace)
+  (result:maybe (events_trace * a))
+  (local_trace:events_trace) :
+  Tot Type0 =
+  enforced_globally (default_check) (apply_changes s0 local_trace) /\
+  enforced_globally (pi_check) (apply_changes s0 local_trace) /\
+  (match result with
+  | Inl v -> let (s1, r) = v in s1 == (apply_changes s0 local_trace)
+  | Inr _ -> True)
+
+effect M4wp
+  (a:Type)
+  (pi_check : monitorable_prop) 
+  (post : events_trace -> maybe (events_trace * a) -> events_trace -> Type0) =
+  IOStHist a
+    (requires (m4wp_invariant_pre pi_check))
+    (ensures (fun h r le -> m4wp_invariant_post pi_check h r le /\ post h r le))
